Lott/Data/List.lean
@@ -5,6 +5,12 @@ theorem map_singleton_join (xs : List α) : (xs.map fun x => [f x]).join = xs.ma
   | [] => rfl
   | x :: xs' => by rw [List.map, List.map, List.join, List.singleton_append, xs'.map_singleton_join]
 
+theorem not_mem_append' {xs ys : List α} : z ∉ xs ++ ys ↔ z ∉ xs ∧ z ∉ ys where
+  mp zninxsys := ⟨(zninxsys <| mem_append.mpr <| .inl ·), (zninxsys <| mem_append.mpr <| .inr ·)⟩
+  mpr | ⟨xninxs, xninys⟩, xinxsys => match mem_append.mp xinxsys with
+    | .inl xinxs => xninxs xinxs
+    | .inr xinys => xninys xinys
+
 theorem exists_gt (xs : List Nat)
   : ∃ n : Nat, ∀ m : Nat, m ∈ xs → m < n := match xs with
   | [] => .intro 0 fun x' x'in => nomatch x'in
@@ -19,8 +25,7 @@ theorem exists_gt (xs : List Nat)
         split
         · case isTrue h => exact Nat.lt_of_succ_le h
         · case isFalse h => exact Nat.lt_succ_self _
-      | .inr x'inxs' =>
-        Nat.lt_of_lt_of_le (nxs'gt x' x'inxs') <| Nat.le_max_right _ _
+      | .inr x'inxs' => Nat.lt_of_lt_of_le (nxs'gt x' x'inxs') <| Nat.le_max_right _ _
 
 theorem exists_fresh (xs : List Nat) : ∃ n, n ∉ xs :=
   let ⟨nxs, nxsgt⟩ := xs.exists_gt
